theories/ordinals/Ackermann/LNT.v
@@ -53,16 +53,6 @@ Infix "->" := (impH): nt_scope.
 Notation "~ A" := (@notH _ A): nt_scope. 
 Notation "A <-> B" := (@iffH _ A B): nt_scope.
 
-
-Notation k_ t := (apply  (t:Functions _)  (Tnil)).
-
-Notation app1 f arg := 
-  (apply  (f: Functions _)  (Tcons arg (Tnil))).
-About Tnil.
-Notation app2 f arg1 arg2 := 
-  (apply   (f: Functions _) 
-     (Tcons  arg1 (Tcons  arg2 (Tnil)))).
-
 Notation "t = u" := (@equal _ t u): nt_scope.
 Notation "t <> u" := (~ t = u)%nt : nt_scope.
 Notation "'v#' i" := (var i) (at level 3, format "'v#' i") : nt_scope. 
